PiLL/PiLL/Framework/Model/Congruence.lean
@@ -31,7 +31,7 @@ inductive StructCong : Proc → Proc → Prop where
   | par_congr {P P' Q Q' : Proc} :
       StructCong P P' → StructCong Q Q' → StructCong (P |ₚ Q) (P' |ₚ Q')
   | cut_congr {P P' : Proc} :
-      StructCong P P' → StructCong (𝑣⸨#, #⸩ P) (𝑣⸨#, #⸩ P')
+      StructCong P P' → StructCong (𝑣⸨#,#⸩ P) (𝑣⸨#,#⸩ P')
 
   | par_comm (P Q : Proc) : StructCong (P |ₚ Q) (Q |ₚ P)
   | par_assoc (P Q R : Proc) : StructCong ((P |ₚ Q) |ₚ R) (P |ₚ (Q |ₚ R))
@@ -42,7 +42,7 @@ inductive StructCong : Proc → Proc → Prop where
   -- which could risk capturing 0 or 1 from 𝒗⸨#, #⸩. This amounts to checking lcProc Q.
   | cut_scope {P Q : Proc} :
       lcProc0 Q →
-      StructCong ((𝑣⸨#, #⸩ P) |ₚ Q) (𝑣⸨#, #⸩ (P |ₚ Q))
+      StructCong ((𝑣⸨#,#⸩ P) |ₚ Q) (𝑣⸨#,#⸩ (P |ₚ Q))
 
 infix:50 " ≡ₚ " => StructCong
 
